AwsCryptographicMaterialProviders/dafny/AwsCryptographyKeyStore/src/DDBKeystoreOperations.dfy
@@ -10,6 +10,9 @@ module DDBKeystoreOperations {
   import UTF8
   import Structure
 
+  const BRANCH_KEY_NOT_EXIST := "attribute_not_exists(" + Structure.BRANCH_KEY_IDENTIFIER_FIELD + ")"
+  const BRANCH_KEY_EXISTS := "attribute_exists(" + Structure.BRANCH_KEY_IDENTIFIER_FIELD + ")"
+
   method WriteNewKeyToStore(
     versionBranchKeyItem: Structure.VersionBranchKeyItem,
     activeBranchKeyItem: Structure.ActiveBranchKeyItem,
@@ -17,47 +20,35 @@ module DDBKeystoreOperations {
     tableName: DDB.TableName,
     ddbClient: DDB.IDynamoDBClient
   )
-    returns (res: Result<DDB.TransactWriteItemsOutput, Types.Error>)
+    returns (output: Result<DDB.TransactWriteItemsOutput, Types.Error>)
     requires
-      && activeBranchKeyItem[Structure.BRANCH_KEY_IDENTIFIER_FIELD] == versionBranchKeyItem[Structure.BRANCH_KEY_IDENTIFIER_FIELD] == beaconKeyItem[Structure.BRANCH_KEY_IDENTIFIER_FIELD]
+      && activeBranchKeyItem[Structure.BRANCH_KEY_IDENTIFIER_FIELD]
+      == versionBranchKeyItem[Structure.BRANCH_KEY_IDENTIFIER_FIELD]
+      == beaconKeyItem[Structure.BRANCH_KEY_IDENTIFIER_FIELD]
       && activeBranchKeyItem[Structure.BRANCH_KEY_ACTIVE_VERSION_FIELD] == versionBranchKeyItem[Structure.TYPE_FIELD]
     requires ddbClient.ValidState()
     modifies ddbClient.Modifies
     ensures ddbClient.ValidState()
-  // {
-  //   var branchKeyDDBMap := ToBranchKeyItemAttributeMap(branchKeyContext, wrappedBranchKey);
-  //   var branchKeyTransactWriteItem := CreateTransactWritePutItem(branchKeyDDBMap, tableName);
+  {
+    var items: DDB.TransactWriteItemList := [
+      CreateTransactWritePutItem(versionBranchKeyItem, tableName, Some(BRANCH_KEY_NOT_EXIST)),
+      CreateTransactWritePutItem(activeBranchKeyItem, tableName, Some(BRANCH_KEY_NOT_EXIST)),
+      CreateTransactWritePutItem(beaconKeyItem, tableName, Some(BRANCH_KEY_NOT_EXIST))
+    ];
 
-  //   var beaconKeyDDBMap := ToBranchKeyItemAttributeMap(beaconKeyContext, wrappedBeaconKey);
-  //   var beaconKeyTransactWriteItem := CreateTransactWritePutItem(beaconKeyDDBMap, tableName);
+    var transactRequest := DDB.TransactWriteItemsInput(
+      TransactItems := items,
+      ReturnConsumedCapacity := None,
+      ReturnItemCollectionMetrics := None,
+      ClientRequestToken := None
+    );
 
-  //   :- Need(
-  //     // In order to be certain we are writing something that is well formed
-  //     // and something we will be able to get or query we need to ensure it has certain properties
-  //     && validBeaconKeyItem?(beaconKeyDDBMap)
-  //     && validActiveBranchKey?(branchKeyDDBMap),
-  //     Types.KeyStoreException(message := "Unable to write key material to Key Store: " + tableName)
-  //   );
+    var maybeTransactWriteResponse := ddbClient.TransactWriteItems(transactRequest);
+    var transactWriteItemsResponse :- maybeTransactWriteResponse
+    .MapFailure(e => Types.ComAmazonawsDynamodb(ComAmazonawsDynamodb := e));
 
-  //   var items: DDB.TransactWriteItemList := [
-  //     branchKeyTransactWriteItem,
-  //     beaconKeyTransactWriteItem
-  //   ];
-
-  //   var transactRequest := DDB.TransactWriteItemsInput(
-  //     TransactItems := items,
-  //     ReturnConsumedCapacity := None,
-  //     ReturnItemCollectionMetrics := None,
-  //     ClientRequestToken := None
-  //   );
-
-  //   var maybeTransactWriteResponse := ddbClient.TransactWriteItems(transactRequest);
-  //   var transactWriteItemsResponse :- maybeTransactWriteResponse
-  //   .MapFailure(e => Types.ComAmazonawsDynamodb(ComAmazonawsDynamodb := e));
-
-  //   res := Success(transactWriteItemsResponse);
-  // }
-
+    output := Success(transactWriteItemsResponse);
+  }
 
   method WriteNewBranchKeyVersionToKeystore(
     versionBranchKeyItem: Structure.VersionBranchKeyItem,
@@ -65,43 +56,32 @@ module DDBKeystoreOperations {
     tableName: DDB.TableName,
     ddbClient: DDB.IDynamoDBClient
   )
-    returns (res: Result<DDB.TransactWriteItemsOutput, Types.Error>)
+    returns (output: Result<DDB.TransactWriteItemsOutput, Types.Error>)
     requires
       && activeBranchKeyItem[Structure.BRANCH_KEY_IDENTIFIER_FIELD] == versionBranchKeyItem[Structure.BRANCH_KEY_IDENTIFIER_FIELD]
       && activeBranchKeyItem[Structure.BRANCH_KEY_ACTIVE_VERSION_FIELD] == versionBranchKeyItem[Structure.TYPE_FIELD]
     requires ddbClient.ValidState()
     modifies ddbClient.Modifies
     ensures ddbClient.ValidState()
-  // {
-  // var decryptOnlyBranchKeyTransactWriteItem := CreateTransactWritePutItem(decryptOnlyBranchKey, tableName);
-  // var newActiveBranchKeyTransactWriteItem := CreateTransactWritePutItem(newActiveBranchKey, tableName);
+  {
+    var items: DDB.TransactWriteItemList := [
+      CreateTransactWritePutItem(versionBranchKeyItem, tableName, Some(BRANCH_KEY_EXISTS)),
+      CreateTransactWritePutItem(activeBranchKeyItem, tableName, Some(BRANCH_KEY_NOT_EXIST))
+    ];
 
-  // :- Need(
-  //   // In order to be certain we are writing something that is well formed
-  //   // and something we will be able to get or query we need to ensure it has certain properties
-  //   && validActiveBranchKey?(newActiveBranchKey)
-  //   && validVersionBranchKey?(decryptOnlyBranchKey),
-  //   Types.KeyStoreException(message := "Unable to write key material to Key Store: " + tableName)
-  // );
+    var transactRequest := DDB.TransactWriteItemsInput(
+      TransactItems := items,
+      ReturnConsumedCapacity := None,
+      ReturnItemCollectionMetrics := None,
+      ClientRequestToken := None
+    );
 
-  // var items: DDB.TransactWriteItemList := [
-  //   decryptOnlyBranchKeyTransactWriteItem,
-  //   newActiveBranchKeyTransactWriteItem
-  // ];
+    var maybeTransactWriteResponse := ddbClient.TransactWriteItems(transactRequest);
+    var transactWriteItemsResponse :- maybeTransactWriteResponse
+    .MapFailure(e => Types.ComAmazonawsDynamodb(ComAmazonawsDynamodb := e));
 
-  // var transactRequest := DDB.TransactWriteItemsInput(
-  //   TransactItems := items,
-  //   ReturnConsumedCapacity := None,
-  //   ReturnItemCollectionMetrics := None,
-  //   ClientRequestToken := None
-  // );
-
-  // var maybeTransactWriteResponse := ddbClient.TransactWriteItems(transactRequest);
-  // var transactWriteItemsResponse :- maybeTransactWriteResponse
-  // .MapFailure(e => Types.ComAmazonawsDynamodb(ComAmazonawsDynamodb := e));
-
-  // res := Success(transactWriteItemsResponse);
-  // }
+    output := Success(transactWriteItemsResponse);
+  }
 
 
   method GetActiveBranchKeyItem(
@@ -109,11 +89,46 @@ module DDBKeystoreOperations {
     tableName: DDB.TableName,
     ddbClient: DDB.IDynamoDBClient
   )
-    returns (res: Result<Structure.ActiveBranchKeyItem, Types.Error>)
+    returns (output: Result<Structure.ActiveBranchKeyItem, Types.Error>)
     requires DDB.IsValid_TableName(tableName)
     requires ddbClient.ValidState()
     modifies ddbClient.Modifies
     ensures ddbClient.ValidState()
+    ensures output.Success?
+            ==>
+              && output.value[Structure.BRANCH_KEY_IDENTIFIER_FIELD].S == branchKeyIdentifier
+  {
+    var dynamoDbKey: DDB.Key := map[
+      Structure.BRANCH_KEY_IDENTIFIER_FIELD := DDB.AttributeValue.S(branchKeyIdentifier),
+      Structure.TYPE_FIELD := DDB.AttributeValue.S(Structure.BRANCH_KEY_ACTIVE_TYPE)
+    ];
+    var ItemRequest := DDB.GetItemInput(
+      Key := dynamoDbKey,
+      TableName := tableName,
+      AttributesToGet := None,
+      ConsistentRead :=  None,
+      ReturnConsumedCapacity := None,
+      ProjectionExpression := None,
+      ExpressionAttributeNames := None
+    );
+
+    var maybeGetItem := ddbClient.GetItem(ItemRequest);
+    var getItemResponse :- maybeGetItem
+    .MapFailure(e => Types.ComAmazonawsDynamodb(ComAmazonawsDynamodb := e));
+
+    :- Need(
+      getItemResponse.Item.Some?,
+      Types.KeyStoreException( message := "No item found for corresponding branch key identifier.")
+    );
+
+    :- Need(
+      && Structure.ActiveBranchKeyItem?(getItemResponse.Item.value)
+      && getItemResponse.Item.value[Structure.BRANCH_KEY_IDENTIFIER_FIELD].S == branchKeyIdentifier,
+      Types.KeyStoreException( message := "Item found is not a valid active branch key.")
+    );
+
+    output := Success(getItemResponse.Item.value);
+  }
 
   method GetVersionBranchKeyItem(
     branchKeyIdentifier: string,
@@ -121,21 +136,113 @@ module DDBKeystoreOperations {
     tableName: DDB.TableName,
     ddbClient: DDB.IDynamoDBClient
   )
-    returns (res: Result<Structure.VersionBranchKeyItem, Types.Error>)
+    returns (output: Result<Structure.VersionBranchKeyItem, Types.Error>)
     requires DDB.IsValid_TableName(tableName)
     requires ddbClient.ValidState()
     modifies ddbClient.Modifies
     ensures ddbClient.ValidState()
+    ensures output.Success?
+            ==>
+              && output.value[Structure.BRANCH_KEY_IDENTIFIER_FIELD].S == branchKeyIdentifier
+              && output.value[Structure.TYPE_FIELD].S == Structure.BRANCH_KEY_TYPE_PREFIX + branchKeyVersion
+  {
+    var dynamoDbKey: DDB.Key := map[
+      Structure.BRANCH_KEY_IDENTIFIER_FIELD := DDB.AttributeValue.S(branchKeyIdentifier),
+      Structure.TYPE_FIELD := DDB.AttributeValue.S(Structure.BRANCH_KEY_TYPE_PREFIX + branchKeyVersion)
+    ];
+    var ItemRequest := DDB.GetItemInput(
+      Key := dynamoDbKey,
+      TableName := tableName,
+      AttributesToGet := None,
+      ConsistentRead :=  None,
+      ReturnConsumedCapacity := None,
+      ProjectionExpression := None,
+      ExpressionAttributeNames := None
+    );
+
+    var maybeGetItem := ddbClient.GetItem(ItemRequest);
+    var getItemResponse :- maybeGetItem
+    .MapFailure(e => Types.ComAmazonawsDynamodb(ComAmazonawsDynamodb := e));
+
+    :- Need(
+      getItemResponse.Item.Some?,
+      Types.KeyStoreException( message := "No item found for corresponding branch key identifier.")
+    );
+
+    :- Need(
+      && Structure.VersionBranchKeyItem?(getItemResponse.Item.value)
+      && getItemResponse.Item.value[Structure.BRANCH_KEY_IDENTIFIER_FIELD].S == branchKeyIdentifier
+      && getItemResponse.Item.value[Structure.TYPE_FIELD].S == Structure.BRANCH_KEY_TYPE_PREFIX + branchKeyVersion,
+      Types.KeyStoreException( message := "Item found is not a valid branch key version.")
+    );
+
+    output := Success(getItemResponse.Item.value);
+  }
 
   method GetBeaconKeyItem(
     branchKeyIdentifier: string,
     tableName: DDB.TableName,
     ddbClient: DDB.IDynamoDBClient
   )
-    returns (res: Result<Structure.BeaconKeyItem, Types.Error>)
+    returns (output: Result<Structure.BeaconKeyItem, Types.Error>)
     requires DDB.IsValid_TableName(tableName)
     requires ddbClient.ValidState()
     modifies ddbClient.Modifies
     ensures ddbClient.ValidState()
+    ensures output.Success?
+            ==>
+              output.value[Structure.BRANCH_KEY_IDENTIFIER_FIELD].S == branchKeyIdentifier
+  {
+    var dynamoDbKey: DDB.Key := map[
+      Structure.BRANCH_KEY_IDENTIFIER_FIELD := DDB.AttributeValue.S(branchKeyIdentifier),
+      Structure.TYPE_FIELD := DDB.AttributeValue.S(Structure.BEACON_KEY_TYPE_VALUE)
+    ];
+    var ItemRequest := DDB.GetItemInput(
+      Key := dynamoDbKey,
+      TableName := tableName,
+      AttributesToGet := None,
+      ConsistentRead :=  None,
+      ReturnConsumedCapacity := None,
+      ProjectionExpression := None,
+      ExpressionAttributeNames := None
+    );
+
+    var maybeGetItem := ddbClient.GetItem(ItemRequest);
+    var getItemResponse :- maybeGetItem
+    .MapFailure(e => Types.ComAmazonawsDynamodb(ComAmazonawsDynamodb := e));
+
+    :- Need(
+      getItemResponse.Item.Some?,
+      Types.KeyStoreException( message := "No item found for corresponding branch key identifier.")
+    );
+
+    :- Need(
+      && Structure.BeaconKeyItem?(getItemResponse.Item.value)
+      && getItemResponse.Item.value[Structure.BRANCH_KEY_IDENTIFIER_FIELD].S == branchKeyIdentifier,
+      Types.KeyStoreException( message := "Item found is not a valid beacon key.")
+    );
+
+    output := Success(getItemResponse.Item.value);
+  }
+
+  function method CreateTransactWritePutItem(
+    item: DDB.AttributeMap,
+    tableName: DDB.TableName,
+    ConditionExpression: Option<DDB.ConditionExpression> := None
+  ): (output: DDB.TransactWriteItem)
+  {
+    DDB.TransactWriteItem(
+      ConditionCheck := None,
+      Put := Some(DDB.Put(
+                    Item := item,
+                    TableName := tableName,
+                    ConditionExpression := ConditionExpression,
+                    ExpressionAttributeNames := None,
+                    ExpressionAttributeValues := None,
+                    ReturnValuesOnConditionCheckFailure := None)),
+      Delete := None,
+      Update := None
+    )
+  }
 
 }
